theories/caesium/lang.v
@@ -902,12 +902,12 @@ Ltac unfold_common_caesium_defs :=
     aligned_to,
     (*Z.divide,*)
   (* Layout *)
-    ly_size, ly_with_align, ly_align_log, layout_wf,
+    ly_size, ly_with_align, ly_align_log, layout_wf, it_layout,
+  (* Address bounds *)
+    max_alloc_end, min_alloc_start, bytes_per_addr,
   (* Integer bounds *)
     max_int, min_int, int_half_modulus, int_modulus,
     bits_per_int, bytes_per_int, bytes_per_addr_log,
-  (* Address bounds *)
-    max_alloc_end, min_alloc_start, bytes_per_addr,
   (* Other byte-level definitions *)
     bits_per_byte in *.
 
