theories/rust_typing/program_rules.v
@@ -1,7 +1,7 @@
 From stdpp Require Import gmap.
+From caesium Require Import lang proofmode derived lifting.
 From refinedrust Require Export base type lft_contexts annotations ltypes programs.
 From refinedrust Require Import ltype_rules.
-From caesium Require Import lang proofmode derived lifting.
 Set Default Proof Using "Type".
 
 Section typing.
