theories/rust_typing/util.v
@@ -1,6 +1,6 @@
 From Coq Require Import Qcanon.
-From iris.bi Require Import fractional.
 From caesium Require Import derived.
+From iris.bi Require Import fractional.
 From iris.proofmode Require Import tactics.
 From refinedrust Require Export base.
 From iris.prelude Require Import options.
